More migration. About to move synchronisation diagrams to their own file.

concurrency/common/HybridMachine.v
@@ -1,4 +1,6 @@
 From mathcomp.ssreflect Require Import ssreflect seq ssrbool ssrfun.
+Require Import Coq.Classes.Morphisms.
+
 Require Import compcert.common.Memory.
 Require Import compcert.common.AST.     (*for typ*)
 Require Import compcert.common.Values. (*for val*)
@@ -15,6 +17,7 @@ Require Import VST.concurrency.common.threadPool.
 
 Require Import VST.concurrency.common.machine_semantics.
 Require Import VST.concurrency.common.permissions.
+Require Import VST.concurrency.compiler.mem_equiv.
 Require Import VST.concurrency.common.bounded_maps.
 Require Import VST.concurrency.common.addressFiniteMap.
 Require Import VST.concurrency.common.scheduler.
@@ -599,31 +602,9 @@ Module DryHybridMachine.
       exists c, semantics.initial_core semSem 0 m c m' v args /\
            ms = mkPool (Krun c) (getCurPerm m', empty_map).
     Set Printing All.
-    Section HybDryMachineLemmas.
 
-      Lemma build_delta_content_restr: forall d m p Hlt,
-        build_delta_content d (@restrPermMap p m Hlt) = build_delta_content d m.
-      Proof.
-        reflexivity.
-      Qed.
 
-      (*TODO: This lemma should probably be moved. *)
-      Lemma threads_canonical:
-        forall ds m i (cnt:containsThread ds i),
-          mem_compatible ds m ->
-          isCanonical (getThreadR cnt).1 /\
-          isCanonical (getThreadR cnt).2.
-        intros.
-        destruct (compat_th _ _ H cnt);
-          eauto using canonical_lt.
-      Qed.
-      (** most of these lemmas are in DryMachinLemmas*)
 
-      (** *Invariant Lemmas*)
-
-      (** ** Updating the machine state**)
-      (* Many invaraint lemmas were removed from here. *)
-    End HybDryMachineLemmas.
 
 
     Definition install_perm tp m tid (Hcmpt: mem_compatible tp m) (Hcnt: containsThread tp tid) m' :=
@@ -655,6 +636,89 @@ Module DryHybridMachine.
 
     
   End DryHybridMachine.
+
+  
+  
+  Section HybDryMachineLemmas.
+
+    (* Lemmas that don't need semantics/threadpool*)
+    
+      Lemma build_delta_content_restr: forall d m p Hlt,
+        build_delta_content d (@restrPermMap p m Hlt) = build_delta_content d m.
+      Proof.
+        reflexivity.
+      Qed.
+
+      (** Assume some threadwise semantics *)
+      Context {Sem: Semantics}
+            {tpool : @ThreadPool.ThreadPool dryResources Sem}.
+    
+      
+      (*TODO: This lemma should probably be moved. *)
+      Lemma threads_canonical:
+        forall ds m i (cnt:containsThread ds i),
+          mem_compatible ds m ->
+          isCanonical (getThreadR cnt).1 /\
+          isCanonical (getThreadR cnt).2.
+        intros.
+        destruct (compat_th _ _ H cnt);
+          eauto using canonical_lt.
+      Qed.
+      (** most of these lemmas are in DryMachinLemmas*)
+
+      (** *Invariant Lemmas*)
+
+      (** ** Updating the machine state**)
+      (* Many invaraint lemmas were removed from here. *)
+      
+    
+    Notation thread_perms st i cnt:= (fst (@getThreadR _ _ _ st i cnt)).
+    Notation lock_perms st i cnt:= (snd (@getThreadR  _ _ _ st i cnt)).
+    Record thread_compat st i
+           (cnt:containsThread st i) m:=
+      { th_comp: permMapLt (thread_perms _ _ cnt) (getMaxPerm m);
+        lock_comp: permMapLt (lock_perms _ _ cnt) (getMaxPerm m)}.
+    Instance thread_compat_proper st i:
+        Proper (Logic.eq ==> Max_equiv ==> iff) (@thread_compat st i).
+      Proof. setoid_help.proper_iff;
+               setoid_help.proper_intros; subst.
+             constructor.
+             - eapply permMapLt_equiv.
+               reflexivity.
+               symmetry; apply H0.
+               eapply H1.
+             - eapply permMapLt_equiv.
+               reflexivity.
+               symmetry; apply H0.
+               eapply H1.
+      Qed.
+    Lemma mem_compatible_thread_compat:
+      forall (st1 : ThreadPool.t) (m1 : mem) (tid : nat)
+        (cnt1 : containsThread st1 tid),
+        mem_compatible st1 m1 -> thread_compat _ _ cnt1 m1.
+    Proof. intros * H; constructor; apply H. Qed.
+    Lemma mem_compat_Max:
+        forall Sem Tp st m m',
+          Max_equiv m m' ->
+          Mem.nextblock m = Mem.nextblock m' ->
+          @mem_compatible Sem Tp st m ->
+          @mem_compatible Sem Tp st m'.
+      Proof.
+        intros * Hmax Hnb H.
+        assert (Hmax':access_map_equiv (getMaxPerm m) (getMaxPerm m'))
+          by eapply Hmax.
+        constructor; intros;
+          repeat rewrite <- Hmax';
+          try eapply H; eauto.
+        unfold Mem.valid_block; rewrite <- Hnb;
+          eapply H; eauto.
+      Qed.
+
+  End HybDryMachineLemmas.
+  Notation thread_perms st i cnt:= (fst (@getThreadR _ _ _ st i cnt)).
+  Notation lock_perms st i cnt:= (snd (@getThreadR  _ _ _ st i cnt)).
+    
+    
 End DryHybridMachine.
 
 Export DryHybridMachine.
